CODIGO/SETS/SetCover.dfy
@@ -11,3 +11,7 @@ ghost predicate isCover<T>(universe:set<T>, sets:set<set<T>>)
 {
   forall u | u in universe :: (exists s | s in sets :: u in s)
 }
+
+method verifyIsCover<T>(universe:set<T>, sets:set<set<T>>, k:nat, witnes:set<set<T>>) returns (b:bool)
+ensures b == isCover(universe, witnes) && |witnes| <= k 
+ensures b == SetCover(universe, sets, k)
