CODIGO/SUMA/Problems/Envasar.dfy
@@ -7,20 +7,13 @@ include "../Auxiliar/Sum.dfy"
 // tales que la suma de los elementos de cada subconjunto sea a lo sumo E
 ghost predicate Envasar(A:multiset<nat>, E:nat, k:nat)
 { 
-  exists I:multiset<multiset<nat>> | Valid(I,A,E) :: |I| <= k;
+  exists I:multiset<multiset<nat>> :: 
+      forall e | e in I :: e <= A && GSumNat(e) <= E 
+   && |I| <= k && Union(I) == A
 }
 
-/*exists I:multiset<multiset<nat>> | forall e1 | e1 in I :: e1 <= A && GSum(e1) <= E && forall e2 | e2 in I :: e1 * e2 == multiset{}) 
-  :: |I| <= k && Union(I) == A;*/
-
-ghost predicate Valid (I:multiset<multiset<nat>>, A:multiset<nat>, E:nat) : a
+ghost function Union (I:multiset<multiset<nat>>) : multiset<nat>
 {
-  if m == multiset{} then {}
-  else var i :| i in I; i + Union(m - multiset{i})
-}
-
-ghost predicate Union (I:multiset<multiset<nat>>) : multiset<nat>
-{
-  if m == multiset{} then {}
-  else var i :| i in I; i + Union(m - multiset{i})
+  if I == multiset{} then multiset{}
+  else var i :| i in I; i + Union(I-multiset{i})
 }
