CODIGO/SUMA/Transformations/SumaToParticion.dfy
@@ -5,7 +5,7 @@ include "../Problems/Particion.dfy"
 
 function Suma_to_Particion(A:multiset<int>, S:int) : (r:(multiset<int>))
 {
-    var N := 2*S - FSum(A);
+    var N := 2*S - FSumInt(A);
     (A + multiset{N})
 }
 
